Set_Graphs/Graph_Algorithms/DFS_BFS_Export.thy
@@ -1,0 +1,28 @@
+theory DFS_BFS_Export
+  imports DFS_Imperative BFS_Refinement_Instantiation BFS_Example
+begin
+
+export_code
+(*nat transforms*)
+nat_of_integer integer_of_nat
+(*iam for dfs*)
+iam_dfs_imp iam_dfs_initial_state iam_graph_from_list
+(*string hm for dfs*)
+hm_dfs_imp hm_dfs_initial_state hm_graph_from_list 
+(*integer hm for dfs*)
+him_dfs_imp him_dfs_initial_state him_graph_from_list 
+(*functional rbt for dfs*)
+rbt_dfs_initial_state rbt_neighbourhood rbt_dfs_impl rbt_add_edge
+rbt_from_list
+(*dfs state*)
+sstack sseen rreturn rreachable not_reachable
+(*bfs iam*)
+BFS_dag_iam BFS_check_reachable_iam
+(*BFS rbt*) 
+BFS_dag_rbt BFS_check_reachable_rbt build_rbt_sources
+
+in SML_imp module_name exported file_prefix Unweighted_Graph_imperative
+
+
+
+end
